IML/LFPSoundness.lean
@@ -208,8 +208,8 @@ theorem soundness_lfp {Γ : Set (Pattern Symbol)} {φ : Pattern Symbol}
     exact fun _ _ _ _ _ m => hvalid_postFixpoint_lfp hpos m
   | park _ ih =>
     exact fun L _ M hΓ ρ m => hvalid_park_lfp (ih L M hΓ ρ) m
-  | singleton =>
-    exact fun _ _ _ _ _ m => hvalid_singleton m
+  | singletonStrong =>
+    exact fun _ _ _ _ _ m => hvalid_singletonStrong m
   | propagationOrLeft =>
     exact fun _ _ _ _ _ m => hvalid_propagationOrLeft m
   | propagationOrRight =>
